Fixed loop structure

translator/lean/llzk/Llzk/Temp/LoopStructureTest.lean
@@ -5,7 +5,23 @@
 inductive Com where
   | skip : Com
   | cond (t e : List Com) : Com
+  | loope (start rep : Nat ) (body: List Com) : Com
   | loop (start rep : Nat ) (body: List Com) : Com
+
+mutual
+def num_of_loope_p (p : List Com) : Nat :=
+  match p with
+   | [] => 0
+   | c::cs =>
+      num_of_loope_cmd c + num_of_loope_p cs
+def num_of_loope_cmd (c : Com) : Nat :=
+   match c with
+   | Com.skip => 0
+   | Com.cond t e => num_of_loope_p t + num_of_loope_p e
+   | Com.loope _ _ body => 1+num_of_loope_p body
+   | Com.loop _ _ body => num_of_loope_p body
+end
+
 
 /- Size of a program, which is used for proving termination
    of the interpreter and corresponding proofs.
@@ -18,94 +34,140 @@ def size_of_prog (p : List Com) : Nat :=
 
 def size_of_cmd (c: Com) : Nat :=
   match c with
-   | Com.skip => 0
-   | Com.cond t e => size_of_prog t + size_of_prog e
-   | Com.loop _ rep body => rep*(1+(size_of_prog body))
+   | Com.skip => 1
+   | Com.cond t e => 1 + size_of_prog t + size_of_prog e
+   | Com.loope _ _ body => 1 + size_of_prog body
+   | Com.loop _ rep body => rep*(1+size_of_prog body)
 end
+
+theorem num_of_loope_p_cons_1 (c : Com) (cs : List Com) (H: num_of_loope_cmd c = 0) : num_of_loope_p (c :: cs) = num_of_loope_p cs := by
+  simp only [num_of_loope_p]
+  simp only [H]
+  grind
+
+theorem num_of_loope_p_cons_2 (c : Com) (cs : List Com) (H: num_of_loope_p cs = 0) : num_of_loope_p (c :: cs) = num_of_loope_cmd c := by
+  simp only [num_of_loope_p]
+  grind
+
+
+
+def const_eval (a : Nat) : Nat := a
 
 /- This follows the same structure as the interpreter, but instead of executing
    commands, it counts the number of commands in a program. This is
    used to show that we can prove termination.
 -/
+mutual
 def count (p : List Com) : Nat :=
   match p with
-   | [] => 0
-   | c::cs =>
-   let x := match c with
-            | Com.skip => 0
-            | Com.cond t e => 0 + count t + count e
-            | Com.loop start rep body =>
-              if rep > 0 then
-                0 + count body + count [(Com.loop (start+1) (rep-1) body)]
-              else
-                0
-    x + count cs
-termination_by
-  size_of_prog p
+  | [] => 1
+  | c::cs =>
+    count_cmd c + count cs
+termination_by (num_of_loope_p p, size_of_prog p)
 decreasing_by
-  · simp only [size_of_prog, size_of_cmd]
+  · have h1 : num_of_loope_cmd c ≤ num_of_loope_cmd c + num_of_loope_p cs := by
+      grind
+    rcases Nat.lt_or_eq_of_le h1 with h_less | h_equal
+    · simp only [num_of_loope_p]
+      apply Prod.Lex.left
+      exact h_less
+    · simp only [num_of_loope_p]
+      rw [← h_equal]
+      apply Prod.Lex.right
+      simp only [size_of_prog]
+      grind
+  · have h1 : num_of_loope_p cs ≤ num_of_loope_cmd c + num_of_loope_p cs := by
+      grind
+    rcases Nat.lt_or_eq_of_le h1 with h_less | h_equal
+    · simp only [num_of_loope_p]
+      apply Prod.Lex.left
+      exact h_less
+    · simp only [num_of_loope_p]
+      rw [← h_equal]
+      apply Prod.Lex.right
+      simp only [size_of_prog]
+      grind
+
+def count_cmd (c : Com) : Nat :=
+  match c with
+  | Com.skip => 1
+  | Com.cond t e => 1 + count t + count e
+  | Com.loope start rep body =>
+    let start' := const_eval start
+    let rep' := const_eval rep
+    count_cmd (Com.loop start' rep' body)
+  | Com.loop start (rep+1) body =>
+      1+count body + count_cmd (Com.loop (start+1) rep body)
+  | Com.loop _ 0 _ =>
+      1
+termination_by (num_of_loope_cmd c, size_of_cmd c)
+decreasing_by
+  · have h1 : num_of_loope_p t ≤ num_of_loope_p t +  num_of_loope_p e := by grind
+    simp only [num_of_loope_cmd]
+    rcases Nat.lt_or_eq_of_le h1 with h_less | h_equal
+    · apply Prod.Lex.left
+      exact h_less
+    · rw [← h_equal]
+      apply Prod.Lex.right
+      simp only [size_of_cmd]
+      grind
+  · have h1 : num_of_loope_p e ≤ num_of_loope_p t +  num_of_loope_p e := by grind
+    simp only [num_of_loope_cmd]
+    rcases Nat.lt_or_eq_of_le h1 with h_less | h_equal
+    · apply Prod.Lex.left
+      exact h_less
+    · rw [← h_equal]
+      apply Prod.Lex.right
+      simp only [size_of_cmd]
+      grind
+  · apply Prod.Lex.left
+    simp only [num_of_loope_cmd]
     grind
-  · simp only [size_of_prog, size_of_cmd]
+  · simp only [num_of_loope_cmd]
+    apply Prod.Lex.right
+    simp only [size_of_cmd]
     grind
-  · simp only [size_of_prog, size_of_cmd]
-    rename_i h_rep
-    rw [← Nat.sub_add_cancel h_rep]
+  · simp only [num_of_loope_cmd]
+    apply Prod.Lex.right
+    simp only [size_of_cmd]
     grind
-  · simp only [size_of_prog, size_of_cmd]
-    rename_i h_rep
-    rw [← Nat.sub_add_cancel h_rep]
+end
+
+
+mutual
+theorem count_nonneg (p : List Com) : count p > 0 := by
+  induction p with
+  | nil =>
+    simp only [count]
     grind
-  · simp [size_of_prog]
+  | cons c cs ih =>
+    simp only [count]
+    have h1 : count_cmd c > 0 := count_cmd_nonneg c
     grind
 
-/- A simple test to show that we can prove inductive properties
-    about the count function, which is used to show that we can
-    prove termination of inductive principles, etc.
--/
-theorem count_is_zero (p : List Com) : count p = 0 := by
-  cases p with
-  | nil => simp [count]
-  | cons c cs =>
-    cases c with
-    | skip =>
-      simp only [count]
-      have ih : count cs = 0 := count_is_zero cs
-      rw [ih]
-    | cond t e =>
-      simp only[count]
-      have ih_t : count t = 0 := count_is_zero t
-      have ih_e : count e = 0 := count_is_zero e
-      have ih : count cs = 0 := count_is_zero cs
-      rw [ih, ih_t, ih_e ]
-    | loop start rep body =>
-      have ih : count cs = 0 := count_is_zero cs
-      rw [count]
-      by_cases h_rep : rep > 0
-      · simp only [h_rep]
-        simp
-        have ih_body : count body = 0 := count_is_zero body
-        have ih_loop : count [(Com.loop (start+1) (rep-1) body)] = 0
-             := count_is_zero [(Com.loop (start+1) (rep-1) body)]
-        simp [ih, ih_body, ih_loop]
-      · simp only [h_rep]
-        simp
-        simp [ih]
-termination_by
-  size_of_prog p
-decreasing_by
-  · simp only [size_of_prog, size_of_cmd]
+theorem count_cmd_nonneg (c : Com) : count_cmd c > 0 := by
+  cases c with
+  | skip =>
+    simp only [count_cmd]
     grind
-  · simp only [size_of_prog, size_of_cmd]
+  | cond t e =>
+    simp only [count_cmd]
     grind
-  · simp only [size_of_prog, size_of_cmd]
-    grind
-  · simp only [size_of_prog, size_of_cmd]
-    grind
-  · simp only [size_of_prog, size_of_cmd]
-    grind
-  · simp only [size_of_prog, size_of_cmd]
-    rw [← Nat.sub_add_cancel h_rep]
-    grind
-  · simp only [size_of_prog, size_of_cmd]
-    rw [← Nat.sub_add_cancel h_rep]
-    grind
+  | loope start rep body =>
+    simp only [count_cmd]
+    cases (const_eval rep) with
+    | zero =>
+      simp only [count_cmd]
+      grind
+    | succ rep' =>
+      simp only [count_cmd]
+      grind
+  | loop start rep body =>
+    cases rep with
+    | zero =>
+      simp only [count_cmd]
+      grind
+    | succ rep' =>
+      simp only [count_cmd]
+      grind
+end
